@prefix dcterms: <http://purl.org/dc/terms/> .
@prefix m0: <https://raw.githubusercontent.com/aladas-org/cryptocalc/master/system-models/poclets/yggdrasil/M0_Yggdrasil.jsonld#> .
@prefix m3: <M3_GenesisSpace.jsonld#> .
@prefix owl: <http://www.w3.org/2002/07/owl#> .
@prefix rdfs: <http://www.w3.org/2000/01/rdf-schema#> .
@prefix skos: <http://www.w3.org/2004/02/skos/core#> .
@prefix xsd: <http://www.w3.org/2001/XMLSchema#> .

<https://raw.githubusercontent.com/aladas-org/cryptocalc/master/system-models/poclets/yggdrasil/M0_Yggdrasil.jsonld#yggdrasil:Baldr> a owl:NamedIndividual,
        <m1:mythology:MajorDeity> ;
    rdfs:label "Baldr" ;
    m0:cosmicRole "Light, Purity, Beauty" ;
    m0:instantiatesM2 "m2:Agent",
        "m2:Identity",
        "m2:Role" ;
    m0:residesInWorld "m0:yggdrasil:World_Asgard" .

<https://raw.githubusercontent.com/aladas-org/cryptocalc/master/system-models/poclets/yggdrasil/M0_Yggdrasil.jsonld#yggdrasil:Bifrost> a owl:NamedIndividual,
        <m1:mythology:MythicalPlace> ;
    rdfs:label "Bifröst - Rainbow Bridge" ;
    rdfs:comment "Rainbow bridge connecting Midgard to Asgard. Guarded by Heimdall (Gatekeeper). Acts as Interface (enables passage) constrained by Heimdall's enforcement. Destroyed at Ragnarok when Surtr's fire giants cross it." ;
    m0:function "Connection Midgard ↔ Asgard" ;
    m0:gatekeeperRole "Interface component of Heimdall's Gatekeeper pattern" ;
    m0:guardian "m0:yggdrasil:Heimdall" ;
    m0:instantiatesM2 "m2:Interface",
        "m2:Structure" ;
    m0:ragnarokFate "Destroyed when Surtr crosses (Gatekeeper barrier fails)" .

<https://raw.githubusercontent.com/aladas-org/cryptocalc/master/system-models/poclets/yggdrasil/M0_Yggdrasil.jsonld#yggdrasil:Draupnir> a owl:NamedIndividual,
        <m1:mythology:MythicalArtifact> ;
    rdfs:label "Draupnir" ;
    m0:function "Odin's ring, self-replicates every 9 nights" ;
    m0:instantiatesM2 "m2:Identity" .

<https://raw.githubusercontent.com/aladas-org/cryptocalc/master/system-models/poclets/yggdrasil/M0_Yggdrasil.jsonld#yggdrasil:Eagle> a owl:NamedIndividual,
        <m1:mythology:MagicalBird> ;
    rdfs:label "Eagle" ;
    m0:instantiatesM2 "m2:Identity" ;
    m0:systemRole "Omniscient observer at crown" .

<https://raw.githubusercontent.com/aladas-org/cryptocalc/master/system-models/poclets/yggdrasil/M0_Yggdrasil.jsonld#yggdrasil:Fenrir> a owl:NamedIndividual,
        <m1:mythology:MonstrousWolf> ;
    rdfs:label "Fenrir" ;
    m0:instantiatesM2 "m2:Identity" ;
    m0:systemRole "Chaos wolf, bound until Ragnarok" .

<https://raw.githubusercontent.com/aladas-org/cryptocalc/master/system-models/poclets/yggdrasil/M0_Yggdrasil.jsonld#yggdrasil:Freyja> a owl:NamedIndividual,
        <m1:mythology:MajorDeity> ;
    rdfs:label "Freyja" ;
    m0:cosmicRole "Love, Beauty, War, Magic" ;
    m0:instantiatesM2 "m2:Agent",
        "m2:Identity",
        "m2:Role" ;
    m0:residesInWorld "m0:yggdrasil:World_Vanaheim" .

<https://raw.githubusercontent.com/aladas-org/cryptocalc/master/system-models/poclets/yggdrasil/M0_Yggdrasil.jsonld#yggdrasil:Freyr> a owl:NamedIndividual,
        <m1:mythology:MajorDeity> ;
    rdfs:label "Freyr" ;
    m0:cosmicRole "Fertility, Prosperity, Peace" ;
    m0:instantiatesM2 "m2:Agent",
        "m2:Identity",
        "m2:Role" ;
    m0:residesInWorld "m0:yggdrasil:World_Vanaheim" .

<https://raw.githubusercontent.com/aladas-org/cryptocalc/master/system-models/poclets/yggdrasil/M0_Yggdrasil.jsonld#yggdrasil:Frigg> a owl:NamedIndividual,
        <m1:mythology:MajorDeity> ;
    rdfs:label "Frigg" ;
    m0:cosmicRole "Marriage, Motherhood, Foresight" ;
    m0:instantiatesM2 "m2:Agent",
        "m2:Identity",
        "m2:Role" ;
    m0:residesInWorld "m0:yggdrasil:World_Asgard" .

<https://raw.githubusercontent.com/aladas-org/cryptocalc/master/system-models/poclets/yggdrasil/M0_Yggdrasil.jsonld#yggdrasil:Gungnir> a owl:NamedIndividual,
        <m1:mythology:MythicalArtifact> ;
    rdfs:label "Gungnir" ;
    m0:function "Odin's spear, never misses" ;
    m0:instantiatesM2 "m2:Identity" .

<https://raw.githubusercontent.com/aladas-org/cryptocalc/master/system-models/poclets/yggdrasil/M0_Yggdrasil.jsonld#yggdrasil:Heimdall> a owl:NamedIndividual,
        <m1:mythology:MajorDeity> ;
    rdfs:label "Heimdall" ;
    m0:cosmicRole "Guardian of Bifrost" ;
    m0:exemplifiesPattern "m1:mythology:Gatekeeper" ;
    m0:instantiatesM2 "m2:Agent",
        "m2:Identity",
        "m2:Role" ;
    m0:residesInWorld "m0:yggdrasil:World_Asgard" .

<https://raw.githubusercontent.com/aladas-org/cryptocalc/master/system-models/poclets/yggdrasil/M0_Yggdrasil.jsonld#yggdrasil:Hel> a owl:NamedIndividual,
        <m1:mythology:ChthonianDeity> ;
    rdfs:label "Hel" ;
    m0:cosmicRole "Underworld, Death" ;
    m0:instantiatesM2 "m2:Agent",
        "m2:Identity",
        "m2:Role" ;
    m0:residesInWorld "m0:yggdrasil:World_Helheim" .

<https://raw.githubusercontent.com/aladas-org/cryptocalc/master/system-models/poclets/yggdrasil/M0_Yggdrasil.jsonld#yggdrasil:HuginMunin> a owl:NamedIndividual,
        <m1:mythology:MagicalBird> ;
    rdfs:label "HuginMunin" ;
    m0:instantiatesM2 "m2:Identity" ;
    m0:systemRole "Odin's ravens, thought and memory" .

<https://raw.githubusercontent.com/aladas-org/cryptocalc/master/system-models/poclets/yggdrasil/M0_Yggdrasil.jsonld#yggdrasil:Idun> a owl:NamedIndividual,
        <m1:mythology:MinorDeity> ;
    rdfs:label "Idun" ;
    m0:cosmicRole "Youth, Apples of Immortality" ;
    m0:instantiatesM2 "m2:Agent",
        "m2:Identity",
        "m2:Role" ;
    m0:residesInWorld "m0:yggdrasil:World_Asgard" .

<https://raw.githubusercontent.com/aladas-org/cryptocalc/master/system-models/poclets/yggdrasil/M0_Yggdrasil.jsonld#yggdrasil:Jormungandr> a owl:NamedIndividual,
        <m1:mythology:Serpent> ;
    rdfs:label "Jormungandr" ;
    m0:instantiatesM2 "m2:Identity" ;
    m0:systemRole "World serpent, encircles Midgard" .

<https://raw.githubusercontent.com/aladas-org/cryptocalc/master/system-models/poclets/yggdrasil/M0_Yggdrasil.jsonld#yggdrasil:Loki> a owl:NamedIndividual,
        <m1:mythology:MajorDeity> ;
    rdfs:label "Loki" ;
    m0:cosmicRole "Trickster, Chaos, Transformation" ;
    m0:exemplifiesPattern "m1:mythology:Trickster" ;
    m0:instantiatesM2 "m2:Agent",
        "m2:Identity",
        "m2:Role" ;
    m0:residesInWorld "m0:yggdrasil:World_Asgard" .

<https://raw.githubusercontent.com/aladas-org/cryptocalc/master/system-models/poclets/yggdrasil/M0_Yggdrasil.jsonld#yggdrasil:Mjolnir> a owl:NamedIndividual,
        <m1:mythology:MythicalArtifact> ;
    rdfs:label "Mjolnir" ;
    m0:function "Thor's hammer, returns when thrown" ;
    m0:instantiatesM2 "m2:Identity" .

<https://raw.githubusercontent.com/aladas-org/cryptocalc/master/system-models/poclets/yggdrasil/M0_Yggdrasil.jsonld#yggdrasil:Nidhogg> a owl:NamedIndividual,
        <m1:mythology:Dragon> ;
    rdfs:label "Nidhogg" ;
    m0:instantiatesM2 "m2:Identity" ;
    m0:systemRole "Gnaws roots, degradation agent" .

<https://raw.githubusercontent.com/aladas-org/cryptocalc/master/system-models/poclets/yggdrasil/M0_Yggdrasil.jsonld#yggdrasil:Njord> a owl:NamedIndividual,
        <m1:mythology:MajorDeity> ;
    rdfs:label "Njord" ;
    m0:cosmicRole "Sea, Wind, Wealth" ;
    m0:instantiatesM2 "m2:Agent",
        "m2:Identity",
        "m2:Role" ;
    m0:residesInWorld "m0:yggdrasil:World_Vanaheim" .

<https://raw.githubusercontent.com/aladas-org/cryptocalc/master/system-models/poclets/yggdrasil/M0_Yggdrasil.jsonld#yggdrasil:Nornes> a owl:NamedIndividual,
        <m1:mythology:CosmicForce> ;
    rdfs:label "Nornes - The Three Fates" ;
    rdfs:comment "Collective cosmic force: three fate weavers (Urd=Past, Verdandi=Present, Skuld=Future). Water Yggdrasil's roots from Urd's well, maintaining system equilibrium. Represent restorative aspect of CyclicTension (opposite Nidhogg's degradation)." ;
    skos:altLabel "The Fates",
        "Urd, Verdandi, Skuld" ;
    m0:associatedPole "m0:yggdrasil:Pole_7_Synthesis" ;
    m0:collectiveFunction "Fate weaving, system restoration, equilibrium maintenance" ;
    m0:cyclicTensionRole "Restorative agent (opposed to Nidhogg's degradation)" ;
    m0:instantiatesM1Pattern "m1:core:CyclicTension" ;
    m0:instantiatesM2 "m2:Agent",
        "m2:Role" ;
    m0:location "m0:yggdrasil:World_Asgard" ;
    m0:members "Skuld (Future/Debt)",
        "Urd (Past/Origin)",
        "Verdandi (Present/Becoming)" .

<https://raw.githubusercontent.com/aladas-org/cryptocalc/master/system-models/poclets/yggdrasil/M0_Yggdrasil.jsonld#yggdrasil:Odin> a owl:NamedIndividual,
        <m1:mythology:SupremeDeity> ;
    rdfs:label "Odin" ;
    m0:cosmicRole "Wisdom, War, Poetry, Magic" ;
    m0:instantiatesM2 "m2:Agent",
        "m2:Identity",
        "m2:Role" ;
    m0:residesInWorld "m0:yggdrasil:World_Asgard" .

<https://raw.githubusercontent.com/aladas-org/cryptocalc/master/system-models/poclets/yggdrasil/M0_Yggdrasil.jsonld#yggdrasil:Pole_1_Origins> a owl:NamedIndividual,
        <https://raw.githubusercontent.com/aladas-org/cryptocalc/master/system-models/poclets/yggdrasil/M0_Yggdrasil.jsonld#yggdrasil:Pole> ;
    rdfs:label "Pole 1: Origins/Memory" ;
    rdfs:comment "Primordial origins, memory, ice/mist. Source of Hvergelmir spring. Foundation of cosmic memory and ancestral origins." ;
    m0:associatedElements "Ice",
        "Mist",
        "Primordial Waters" ;
    m0:function "Origins, Memory, Primordial Source" ;
    m0:keyLocation "Hvergelmir (source spring)" ;
    m0:polarity "Cold/Static" .

<https://raw.githubusercontent.com/aladas-org/cryptocalc/master/system-models/poclets/yggdrasil/M0_Yggdrasil.jsonld#yggdrasil:Pole_2_Formation> a owl:NamedIndividual,
        <https://raw.githubusercontent.com/aladas-org/cryptocalc/master/system-models/poclets/yggdrasil/M0_Yggdrasil.jsonld#yggdrasil:Pole> ;
    rdfs:label "Pole 2: Formation" ;
    rdfs:comment "Crafting, creation, formation of artifacts and structures. Dwarven smithwork, material shaping." ;
    m0:associatedElements "Craft",
        "Metal",
        "Stone" ;
    m0:function "Formation, Crafting, Material Creation" ;
    m0:inhabitants "Dwarves (smiths, craftsmen)" ;
    m0:polarity "Creative/Material" .

<https://raw.githubusercontent.com/aladas-org/cryptocalc/master/system-models/poclets/yggdrasil/M0_Yggdrasil.jsonld#yggdrasil:Pole_3_Impulse> a owl:NamedIndividual,
        <https://raw.githubusercontent.com/aladas-org/cryptocalc/master/system-models/poclets/yggdrasil/M0_Yggdrasil.jsonld#yggdrasil:Pole> ;
    rdfs:label "Pole 3: Impulse" ;
    rdfs:comment "Fire, energy, impulse, dynamic force. Opposite of Niflheim. Creative/destructive heat." ;
    m0:associatedElements "Energy",
        "Fire",
        "Heat" ;
    m0:function "Impulse, Energy, Heat" ;
    m0:keyEntity "Surtr (fire giant)" ;
    m0:polarity "Hot/Dynamic" .

<https://raw.githubusercontent.com/aladas-org/cryptocalc/master/system-models/poclets/yggdrasil/M0_Yggdrasil.jsonld#yggdrasil:Pole_4_Manifestation> a owl:NamedIndividual,
        <https://raw.githubusercontent.com/aladas-org/cryptocalc/master/system-models/poclets/yggdrasil/M0_Yggdrasil.jsonld#yggdrasil:Pole> ;
    rdfs:label "Pole 4: Manifestation" ;
    rdfs:comment "Central vertical axis: Midgard (humans), Asgard (gods), Vanaheim (Vanir). Manifestation of cosmic order in material/divine/natural planes." ;
    m0:function "Manifestation, Vertical Integration, Cosmic Order" ;
    m0:polarity "Balanced/Central" ;
    m0:structure "Vertical axis (3 realms stacked)" .

<https://raw.githubusercontent.com/aladas-org/cryptocalc/master/system-models/poclets/yggdrasil/M0_Yggdrasil.jsonld#yggdrasil:Pole_5_Wisdom> a owl:NamedIndividual,
        <https://raw.githubusercontent.com/aladas-org/cryptocalc/master/system-models/poclets/yggdrasil/M0_Yggdrasil.jsonld#yggdrasil:Pole> ;
    rdfs:label "Pole 5: Wisdom" ;
    rdfs:comment "Ancient wisdom, chaos knowledge, giants' lore. Mimir's well of wisdom. Adversarial wisdom (opposition to gods)." ;
    m0:associatedElements "Chaos",
        "Knowledge",
        "Opposition" ;
    m0:function "Wisdom, Ancient Knowledge, Chaos Lore" ;
    m0:inhabitants "Jotnar (giants)" ;
    m0:keyLocation "Mimisbrunnr (Mimir's well)" ;
    m0:polarity "Wise/Chaotic" .

<https://raw.githubusercontent.com/aladas-org/cryptocalc/master/system-models/poclets/yggdrasil/M0_Yggdrasil.jsonld#yggdrasil:Pole_6_Inspiration> a owl:NamedIndividual,
        <https://raw.githubusercontent.com/aladas-org/cryptocalc/master/system-models/poclets/yggdrasil/M0_Yggdrasil.jsonld#yggdrasil:Pole> ;
    rdfs:label "Pole 6: Inspiration" ;
    rdfs:comment "Light, inspiration, beauty, creativity. Light elves, artistic/spiritual inspiration." ;
    m0:associatedElements "Art",
        "Beauty",
        "Light" ;
    m0:function "Inspiration, Light, Beauty" ;
    m0:inhabitants "Light Elves" ;
    m0:polarity "Luminous/Creative" .

<https://raw.githubusercontent.com/aladas-org/cryptocalc/master/system-models/poclets/yggdrasil/M0_Yggdrasil.jsonld#yggdrasil:Pole_7_Synthesis> a owl:NamedIndividual,
        <https://raw.githubusercontent.com/aladas-org/cryptocalc/master/system-models/poclets/yggdrasil/M0_Yggdrasil.jsonld#yggdrasil:Pole> ;
    rdfs:label "Pole 7: Synthesis" ;
    rdfs:comment "Meta-level synthesis: Tree Crown (Eagle observer) + Urd's Well (Nornes weave fate). Observes entire system, maintains equilibrium through restoration." ;
    m0:function "Synthesis, Observation, Fate Weaving, System Maintenance" ;
    m0:isMetaLevel true ;
    m0:keyEntities "Eagle (observer)",
        "Nornes (fate weavers)" ;
    m0:keyLocations "Tree Crown",
        "Urdarbrunnr (Urd's well)" ;
    m0:polarity "Meta/Synthetic" .

<https://raw.githubusercontent.com/aladas-org/cryptocalc/master/system-models/poclets/yggdrasil/M0_Yggdrasil.jsonld#yggdrasil:Ragnarok> a owl:NamedIndividual,
        <https://raw.githubusercontent.com/aladas-org/cryptocalc/master/system-models/poclets/yggdrasil/M0_Yggdrasil.jsonld#yggdrasil:CatastrophicEvent> ;
    rdfs:label "Ragnarök - Twilight of the Gods" ;
    dcterms:created "2026-02-04" ;
    dcterms:creator "Echopraxium with the collaboration of Claude AI" ;
    rdfs:comment "Catastrophic system bifurcation and fragmentation. Cosmic-scale destruction and renewal. Instantiates CatastrophicBifurcation (M1_CoreConcepts) = MetaconceptCombo(Bifurcation, Fission). Threshold-triggered violent system transformation with no return path to pre-catastrophe state." ;
    m0:asfidProfile [ ] ;
    m0:cyclicInterpretation "Not terminal end but cosmic renewal. World dies and is reborn. Ragnarok = ultimate CyclicTension at cosmic scale. New world emerges from ashes." ;
    m0:dimensions [ ] ;
    m0:instantiatesM1Concept "m1:core:CatastrophicBifurcation" ;
    m0:instantiatesMetaconcept "m2:MetaconceptCombo" ;
    m0:metaconceptComboParents "m2:Bifurcation",
        "m2:Fission" ;
    m0:survivors "Baldr (returns from Hel)",
        "Hodr (Baldr's brother)",
        "Lif and Lifthrasir (human couple, repopulate)",
        "Modi and Magni (Thor's sons, inherit Mjolnir)",
        "Vali (Odin's son)",
        "Vidarr (Odin's son, avenges father)" ;
    m0:systemicRole "Tests maximum stress capacity of Yggdrasil system. CyclicTension (Nidhogg-Nornes) maintains system daily; CatastrophicBifurcation (Ragnarok) destroys and renews system cosmically." ;
    m0:tensorFormula "S⊗D⊗F" ;
    m0:transformationPhase [ ] ;
    m0:triggerMechanism "AND logic - all 5 triggers must occur" ;
    m0:triggers [ ],
        [ ],
        [ ],
        [ ],
        [ ] .

<https://raw.githubusercontent.com/aladas-org/cryptocalc/master/system-models/poclets/yggdrasil/M0_Yggdrasil.jsonld#yggdrasil:Ratatosk> a owl:NamedIndividual,
        <m1:mythology:Messenger> ;
    rdfs:label "Ratatosk" ;
    m0:exemplifiesPattern "m2:Mediator" ;
    m0:instantiatesM2 "m2:Identity" ;
    m0:systemRole "Squirrel, information mediator" .

<https://raw.githubusercontent.com/aladas-org/cryptocalc/master/system-models/poclets/yggdrasil/M0_Yggdrasil.jsonld#yggdrasil:Sleipnir> a owl:NamedIndividual,
        <m1:mythology:HybridCreature> ;
    rdfs:label "Sleipnir" ;
    m0:instantiatesM2 "m2:Identity" ;
    m0:systemRole "8-legged horse, Odin's mount" .

<https://raw.githubusercontent.com/aladas-org/cryptocalc/master/system-models/poclets/yggdrasil/M0_Yggdrasil.jsonld#yggdrasil:Thor> a owl:NamedIndividual,
        <m1:mythology:MajorDeity> ;
    rdfs:label "Thor" ;
    m0:cosmicRole "Thunder, Strength, Protection" ;
    m0:instantiatesM2 "m2:Agent",
        "m2:Identity",
        "m2:Role" ;
    m0:residesInWorld "m0:yggdrasil:World_Asgard" .

<https://raw.githubusercontent.com/aladas-org/cryptocalc/master/system-models/poclets/yggdrasil/M0_Yggdrasil.jsonld#yggdrasil:Tyr> a owl:NamedIndividual,
        <m1:mythology:MajorDeity> ;
    rdfs:label "Tyr" ;
    m0:cosmicRole "War, Justice, Law" ;
    m0:instantiatesM2 "m2:Agent",
        "m2:Identity",
        "m2:Role" ;
    m0:residesInWorld "m0:yggdrasil:World_Asgard" .

<https://raw.githubusercontent.com/aladas-org/cryptocalc/master/system-models/poclets/yggdrasil/M0_Yggdrasil.jsonld#yggdrasil:World_Alfheim> a owl:NamedIndividual,
        <https://raw.githubusercontent.com/aladas-org/cryptocalc/master/system-models/poclets/yggdrasil/M0_Yggdrasil.jsonld#yggdrasil:World> ;
    rdfs:label "Alfheim - World of Light Elves" ;
    rdfs:comment "Realm of light elves (Ljosalfar). Associated with light, beauty, inspiration. Gift from gods to Freyr." ;
    m0:element "Light, Beauty, Inspiration" ;
    m0:inhabitants "Light Elves (Ljosalfar)" ;
    m0:manifestsAsPole "m0:yggdrasil:Pole_6_Inspiration" .

<https://raw.githubusercontent.com/aladas-org/cryptocalc/master/system-models/poclets/yggdrasil/M0_Yggdrasil.jsonld#yggdrasil:World_Asgard> a owl:NamedIndividual,
        <https://raw.githubusercontent.com/aladas-org/cryptocalc/master/system-models/poclets/yggdrasil/M0_Yggdrasil.jsonld#yggdrasil:World> ;
    rdfs:label "Asgard - World of Aesir Gods" ;
    rdfs:comment "Realm of Aesir gods. Contains Valhalla, Odin's hall. Connected to Midgard via Bifrost (guarded by Heimdall)." ;
    m0:element "Divine, Sky, Order" ;
    m0:inhabitants "Aesir gods" ;
    m0:keyLocations "Bifrost entrance",
        "Valhalla" ;
    m0:manifestsAsPole "m0:yggdrasil:Pole_4_Manifestation" .

<https://raw.githubusercontent.com/aladas-org/cryptocalc/master/system-models/poclets/yggdrasil/M0_Yggdrasil.jsonld#yggdrasil:World_Helheim> a owl:NamedIndividual,
        <https://raw.githubusercontent.com/aladas-org/cryptocalc/master/system-models/poclets/yggdrasil/M0_Yggdrasil.jsonld#yggdrasil:World> ;
    rdfs:label "Helheim - World of the Dead" ;
    rdfs:comment "Underworld realm ruled by Hel. Destination for those who die of sickness or old age (not battle)." ;
    m0:element "Death, Underworld" ;
    m0:manifestsAsPole "m0:yggdrasil:Pole_1_Origins" ;
    m0:ruler "m0:yggdrasil:Hel" .

<https://raw.githubusercontent.com/aladas-org/cryptocalc/master/system-models/poclets/yggdrasil/M0_Yggdrasil.jsonld#yggdrasil:World_Jotunheim> a owl:NamedIndividual,
        <https://raw.githubusercontent.com/aladas-org/cryptocalc/master/system-models/poclets/yggdrasil/M0_Yggdrasil.jsonld#yggdrasil:World> ;
    rdfs:label "Jotunheim - World of Giants" ;
    rdfs:comment "Realm of Jotnar (giants). Contains Mimisbrunnr (Mimir's well of wisdom). Often adversaries of gods but also sources of wisdom." ;
    m0:element "Chaos, Wilderness, Ancient Power" ;
    m0:inhabitants "Jotnar (giants)" ;
    m0:keyLocation "Mimisbrunnr (Mimir's well)" ;
    m0:manifestsAsPole "m0:yggdrasil:Pole_5_Wisdom" .

<https://raw.githubusercontent.com/aladas-org/cryptocalc/master/system-models/poclets/yggdrasil/M0_Yggdrasil.jsonld#yggdrasil:World_Midgard> a owl:NamedIndividual,
        <https://raw.githubusercontent.com/aladas-org/cryptocalc/master/system-models/poclets/yggdrasil/M0_Yggdrasil.jsonld#yggdrasil:World> ;
    rdfs:label "Midgard - World of Humans" ;
    rdfs:comment "Middle realm, home of humanity. Protected by Jormungandr (world serpent). Connected to Asgard via Bifrost." ;
    m0:element "Earth, Material Plane" ;
    m0:inhabitants "Humans" ;
    m0:manifestsAsPole "m0:yggdrasil:Pole_4_Manifestation" ;
    m0:protection "Jormungandr encircles Midgard" .

<https://raw.githubusercontent.com/aladas-org/cryptocalc/master/system-models/poclets/yggdrasil/M0_Yggdrasil.jsonld#yggdrasil:World_Muspellheim> a owl:NamedIndividual,
        <https://raw.githubusercontent.com/aladas-org/cryptocalc/master/system-models/poclets/yggdrasil/M0_Yggdrasil.jsonld#yggdrasil:World> ;
    rdfs:label "Muspellheim - World of Fire" ;
    rdfs:comment "Primordial world of fire, heat, flames. Ruled by fire giant Surtr. Opposite of Niflheim. Surtr will burn the world at Ragnarok." ;
    m0:element "Fire, Heat, Flames" ;
    m0:manifestsAsPole "m0:yggdrasil:Pole_3_Impulse" ;
    m0:ruler "Surtr (fire giant)" .

<https://raw.githubusercontent.com/aladas-org/cryptocalc/master/system-models/poclets/yggdrasil/M0_Yggdrasil.jsonld#yggdrasil:World_Niflheim> a owl:NamedIndividual,
        <https://raw.githubusercontent.com/aladas-org/cryptocalc/master/system-models/poclets/yggdrasil/M0_Yggdrasil.jsonld#yggdrasil:World> ;
    rdfs:label "Niflheim - World of Ice and Mist" ;
    rdfs:comment "Primordial world of ice, cold, mist. Contains Hvergelmir spring. One of two primordial realms (with Muspellheim)." ;
    m0:element "Ice, Mist, Cold" ;
    m0:keyLocation "Hvergelmir" ;
    m0:manifestsAsPole "m0:yggdrasil:Pole_1_Origins" .

<https://raw.githubusercontent.com/aladas-org/cryptocalc/master/system-models/poclets/yggdrasil/M0_Yggdrasil.jsonld#yggdrasil:World_Svartalfheim> a owl:NamedIndividual,
        <https://raw.githubusercontent.com/aladas-org/cryptocalc/master/system-models/poclets/yggdrasil/M0_Yggdrasil.jsonld#yggdrasil:World> ;
    rdfs:label "Svartalfheim/Nidavellir - World of Dwarves" ;
    rdfs:comment "Underground realm of dwarves. Master craftsmen who forged divine artifacts (Mjolnir, Gungnir, Draupnir). Also called Nidavellir." ;
    skos:altLabel "Nidavellir" ;
    m0:element "Stone, Metal, Underground" ;
    m0:inhabitants "Dwarves" ;
    m0:manifestsAsPole "m0:yggdrasil:Pole_2_Formation" .

<https://raw.githubusercontent.com/aladas-org/cryptocalc/master/system-models/poclets/yggdrasil/M0_Yggdrasil.jsonld#yggdrasil:World_Vanaheim> a owl:NamedIndividual,
        <https://raw.githubusercontent.com/aladas-org/cryptocalc/master/system-models/poclets/yggdrasil/M0_Yggdrasil.jsonld#yggdrasil:World> ;
    rdfs:label "Vanaheim - World of Vanir Gods" ;
    rdfs:comment "Realm of Vanir gods (fertility, nature, magic). Originally separate from Aesir, joined after Aesir-Vanir war." ;
    m0:element "Nature, Fertility, Magic" ;
    m0:inhabitants "Vanir gods (Freyja, Freyr, Njord)" ;
    m0:manifestsAsPole "m0:yggdrasil:Pole_4_Manifestation" .

<https://raw.githubusercontent.com/aladas-org/cryptocalc/master/system-models/poclets/yggdrasil/M0_Yggdrasil.jsonld#yggdrasil:Yggdrasil_Poclet> a owl:Ontology ;
    m3:ontologyType <https://raw.githubusercontent.com/aladas-org/cryptocalc/master/ontology/M3_GenesisSpace.jsonld#Poclet> ;
    dcterms:created "2026-01-22" ;
    dcterms:creator "Echopraxium with the collaboration of Claude AI" ;
    dcterms:description "Norse cosmology system centered on Yggdrasil World Tree. Validates TSCG framework through: 7-pole multipolar network, 9 interconnected worlds, cyclic tension (Nidhogg-Nornes), catastrophic bifurcation (Ragnarök), mythological patterns (Trickster/Loki, Gatekeeper/Heimdall). Demonstrates complete M3→M2→M1→M0 hierarchy with 20 Identity instances, 12 deities, 7 creatures, 3 artifacts." ;
    dcterms:modified "2026-02-04" ;
    dcterms:title "TSCG M0 Yggdrasil Poclet" ;
    owl:imports "M1_CoreConcepts.jsonld",
        "M1_extensions/mythology/M1_Mythology.jsonld",
        "M2_MetaConcepts.jsonld" ;
    owl:versionInfo "2.0.0" ;
    m0:changelog [ ] ;
    m0:pocletMetadata [ ] ;
    m0:systemArchitecture [ ] ;
    m0:validationStatus [ ] .

<https://raw.githubusercontent.com/aladas-org/cryptocalc/master/system-models/poclets/yggdrasil/M0_Yggdrasil.jsonld#yggdrasil:associatedWithPole> a owl:ObjectProperty ;
    rdfs:label "associated with pole" ;
    rdfs:domain "m1:mythology:MythologicalEntity" ;
    rdfs:range "m0:yggdrasil:Pole" .

<https://raw.githubusercontent.com/aladas-org/cryptocalc/master/system-models/poclets/yggdrasil/M0_Yggdrasil.jsonld#yggdrasil:hasParent> a owl:ObjectProperty ;
    rdfs:label "has parent" ;
    rdfs:domain "m1:mythology:MythologicalEntity" ;
    rdfs:range "m1:mythology:MythologicalEntity" .

<https://raw.githubusercontent.com/aladas-org/cryptocalc/master/system-models/poclets/yggdrasil/M0_Yggdrasil.jsonld#yggdrasil:interactsWith> a owl:ObjectProperty ;
    rdfs:label "interacts with" ;
    rdfs:domain "m1:mythology:MythologicalEntity" ;
    rdfs:range "m1:mythology:MythologicalEntity" .

<https://raw.githubusercontent.com/aladas-org/cryptocalc/master/system-models/poclets/yggdrasil/M0_Yggdrasil.jsonld#yggdrasil:manifestsAsPole> a owl:ObjectProperty ;
    rdfs:label "manifests as pole" ;
    rdfs:domain "m0:yggdrasil:World" ;
    rdfs:range "m0:yggdrasil:Pole" .

<https://raw.githubusercontent.com/aladas-org/cryptocalc/master/system-models/poclets/yggdrasil/M0_Yggdrasil.jsonld#yggdrasil:residesInWorld> a owl:ObjectProperty ;
    rdfs:label "resides in world" ;
    rdfs:domain "m1:mythology:MythologicalEntity" ;
    rdfs:range "m0:yggdrasil:World" .

<https://raw.githubusercontent.com/aladas-org/cryptocalc/master/system-models/poclets/yggdrasil/M0_Yggdrasil.jsonld#yggdrasil:CatastrophicEvent> a owl:Class ;
    rdfs:label "Catastrophic Event" ;
    rdfs:comment "System-scale destructive transformation. Instantiates m1:core:CatastrophicBifurcation." ;
    m0:instantiatesM1Concept "m1:core:CatastrophicBifurcation" .

<https://raw.githubusercontent.com/aladas-org/cryptocalc/master/system-models/poclets/yggdrasil/M0_Yggdrasil.jsonld#yggdrasil:Pole> a owl:Class ;
    rdfs:label "Pole (Functional Node)" ;
    rdfs:comment "Functional node in 7-pole multipolar network. Represents distinct systemic function. Multiple spatial worlds may manifest as single functional pole." ;
    m0:instantiatesM1Concept "m1:core:MultipolarNetwork" ;
    m0:totalPoles 7 .

<https://raw.githubusercontent.com/aladas-org/cryptocalc/master/system-models/poclets/yggdrasil/M0_Yggdrasil.jsonld#yggdrasil:World> a owl:Class ;
    rdfs:label "World (Spatial Realm)" ;
    rdfs:comment "Spatial realm in Norse 9-world cosmology (Niu Heimar). Each world is distinct environment that manifests systemically as one of 7 functional poles." ;
    rdfs:subClassOf "m1:mythology:MythicalPlace" ;
    m0:totalWorlds 9 .

